If $x_0,x_1,\ldots,x_N\in\mathbb{R}$ are distinct, then the cardinal function $p_j(x)$ defined by

$$p_j(x)=\frac{1}{a_j}\prod_{k=0,\neq j}^N(x-x_k),\;\;\;a_j=\prod_{k=0,\neq j}^N(x_j-x_k)$$

is the unique polynomial interpolant of degree $N$ to the values 1 at $x_j$ and 0 at $x_k$, $k\neq j$.
Take the logarithm and differentiate to obtain

$$p_j'(x)=p_j(x)\sum_{k=0,\neq j}^N(x-x_k)^{-1},$$

and derive the formulas

$$D_{ij}=\frac{1}{a_j}\prod_{k=0,\neq j}^N(x_i-x_k)=\frac{a_i}{a_j(x_i-x_j)}\;\;\;(i\neq j)$$

and

$$D_{jj}=\sum_{k=0,\neq j}^N(x_j-x_k)^{-1}$$\\\\

\begin{solution}\renewcommand{\qedsymbol}{}\ \\
    Letting $p_j(x)$ and $a_j$ be as given above, we take the natural logarithm of both sides. This
    gives us

    $$\ln(p_j(x))=\ln(\prod_{k=0,\neq j}^N\frac{(x-x_k)}{(x_j-x_k)})=
    \sum_{k=0,\neq j}^N\ln(\frac{x-x_k}{x_j-x_k})$$

    $$=\sum_{k=0,\neq j}^N\ln(x-x_k)-\sum_{k=0,\neq j}^N\ln(x_j-x_k)$$

    Now differentiating both sides yields

    $$\frac{p'_j(x)}{p_j(x)}=\sum_{k=0,\neq j}^N\frac{1}{(x-x_k)}-0$$

    which gives us the desired equation

    $$p_j'(x)=p_j(x)\sum_{k=0,\neq j}^N(x-x_k)^{-1}$$

\end{solution}   