a. Use exercise 2 to derive an explicit formula for $\sum_{n=0}^{\infty}n^2x^n$.\\

b. Evaluate $\sum_{n=1}^{\infty}\frac{n^2}{2^n}$ and $\sum_{n=1}^{\infty}\frac{n^2}{3^n}$.\\\\

\begin{solution}\renewcommand{\qedsymbol}{}\ \\
    Well, let $f(x)=\sum_{n=0}^{\infty}n^2x^n$. Clearly,
    
    $$f(x)=x\sum_{n=0}^{\infty}n^2x^{n-1}=x\frac{d}{dx}\sum_{n=0}^{\infty}nx^n$$
    $$=x\frac{d}{dx}(\frac{x}{(1-x)^2})=x(\frac{1-x^2}{(1-x)^4})=\frac{x-x^3}{(1-x)^4}$$

    Let $f(x)=\sum_{n=0}^{\infty}n^2x^n$ and first set $x=\frac12$. By the formula derived above, we
    notice that
    
    $$f(\frac12)=\frac{\frac12-(\frac12)^3}{(\frac12)^4}$$
    $$=\frac{\frac12-\frac18}{\frac{1}{16}}=\frac{\frac38}{{1}{16}}=6$$
    
    Now set $x=\frac13$. By the same formula, we can conclude
    
    $$f(\frac13)=\frac{\frac13-(\frac13)^3}{(\frac23)^4}=\frac{\frac{8}{27}}{\frac{16}{81}}=\frac32$$

\end{solution}