a. Observe $\sum_{n=0}^{\infty}nx^n=\frac{x}{(1-x)^2}$ for $|x|<1$.\\

b. Evaluate $\sum_{n=1}^{\infty}\frac{n}{2^n}$.\\

c. Evaluate $\sum_{n=1}^{\infty}\frac{n}{3^n}$ and $\sum_{n=1}^{\infty}\frac{(-1)^nn}{3^n}$.\\\\

\begin{solution}\renewcommand{\qedsymbol}{}\ \\
    Let $f(x)=\sum_{n=0}^{\infty}nx^n$, for $|x|<1$. Well,
    
    $$f(x)=x\sum_{n=0}^{\infty}nx^{n-1}=x\frac{d}{dx}\sum_{n=0}^{\infty}x^n$$
    $$=x\frac{d}{dx}(\frac{1}{1-x})=x(\frac{1}{(1-x)^2})=\frac{x}{(1-x)^2}$$

    So, let $f(x)=\sum_{n=0}^{\infty}nx^n$. Set $x=\frac12$. So, we get
    
    $$f(\frac12)=\sum_{n=0}^{\infty}n(\frac12)^n$$
    $$=\frac{\frac12}{(1-\frac12)^2}=\frac{\frac12}{\frac14}=2$$

    Again, let $f(x)=\sum_{n=0}^{\infty}nx^n$ and set $x=\frac13$. By the same proces above, we get that
    $f(\frac13)=\frac{\frac13}{\frac49}=\frac34$. Now, set $x=\frac{-1}{3}$. By the same process we get
    $f(\frac{-1}{3})=\frac{\frac{-1}{3}}{\frac{16}{9}}=\frac{-3}{16}$.

\end{solution}