a. Observe $e^{-x^2}=\sum_{n=0}^{\infty}\frac{(-1)^n}{n!}x^{2n}$ for $x\in\mathbb{R}$ since
$e^x=\sum_{n=0}^{\infty}\frac{1}{n!}x^{n}$ for $x\in\mathbb{R}$.\\

b. Express $F(x)=\int_{0}^{x} e^{-t^2} \,dt$ as a power series.\\\\

\begin{solution}\renewcommand{\qedsymbol}{}\ \\
    Well, define $y=-x^2$. Notice we have
    
    $$e^y=\sum_{n=0}^{\infty}\frac{1}{n!}y^{n}=\sum_{n=0}^{\infty}\frac{1}{n!}(-x^2)^{n}$$
    $$=\sum_{n=0}^{\infty}\frac{1}{n!}(-1)^n(x^2)^{n}=\sum_{n=0}^{\infty}\frac{(-1)^n}{n!}x^{2n}$$

    Well,
    
    $$F(x)=\int_{0}^{x} e^{-t^2} \,dt=\int_{0}^{x}\sum_{n=0}^{\infty}\frac{(-1)^n}{n!}t^{2n}\,dt$$
    $$=\sum_{n=0}^{\infty}\frac{(-1)^n}{(n!)(2n+1)}x^{2n+1}$$


\end{solution}