We showed in Example 5.4.4 that $\hat{\sigma}^2=\frac1n\sum_{i=1}^n(Y_i -Y)^2$ is biased for $\sigma^2$.
Suppose $\mu$ is known and does not have to be estimated by $\bar{Y}$. Show that
$\hat{\sigma}^2=\frac1n\sum_{i=1}^n(Y_i-\mu)^2$ is unbiased for $\sigma^2$.\\\\

\begin{solution}\renewcommand{\qedsymbol}{}\ \\
    Well,
    
    $$E(\hat{\sigma}^2)=E(\frac1n\sum_{i=1}^n(Y_i-\mu)^2)=\frac1n\sum_{i=1}^nE((Y_i-\mu^2)^2)$$
    $$=\frac1n\sum_{i=1}^n(\sigma^2)=\frac1n(n\sigma^2)=\sigma^2$$
    
    Thus, we have that $\hat{\sigma}^2$ is an unbiased estimator for $\sigma^2$ as desired.

\end{solution}