Suppose that $(R_1,+_1,\cdot_1)$ and $(R_2,+_2,\cdot_2)$ are rings. We can define operations $+$ and
$\cdot$ on $R_1\times R_2$ by $(x_1,y_1)+(x_2,y_2)=(x_1+_1y_1,x_2+_2y_2)$ and
$(x_1,y_1)\cdot(x_2,y_2)=(x_1\cdot_1y_1,x_2\cdot_2y_2)$. Prove that $R_1\times R_2$ is a ring with
these operations.\\\\

\begin{solution}\renewcommand{\qedsymbol}{}\ \\
    Let $(R_1,+_1,\cdot_1), (R_2,+_2,\cdot_2)$, and $R_1\times R_2$ with operations $+$ and $\cdot$ be
    as above. Now, let $(a,b),(c,d)\in R_1\times R_2$. Then clearly, $R_1\times R_2$ is closed under
    $+$ since $a+b\in R_1$ and $c+d\in R_2$. Now, let $(a,b),(c,d),(e,f)\in R_1\times R_2$. Now,
    
    $$((a,b)+(b,d))+(e,f)=(a+_1c,b+_2d)+(e,f)=((a+_1c)+_1e,(b+_2d)+_2f)=(a+_1(c+_1e),b+_2(d+_2f))$$
    $$=(a,b)+(c+_1e,d+_2f)=(a,b)+((c,d)+(e,f))$$
    
    by associativity of addition on $R_1$ and $R_2$. Next, let $(x,y)\in R_1\times R_2$. Now,
    $(0_1,0_2)\in R_1\times R_2$ where $0_i$ for $i=1,2$ is the identity of $R_i$. So,
    
    $$(x,y)+(0_1,0_2)=(x+_10_1,y+_20_2)=(x,y)=(0_1+_1x,0_2+_2y)=(0_1,0_2)+(x,y)$$
    
    Hence $R_1\times R_2$ has an identity, namely $(0_1,0_2)$. Let $x,y\in R_1\times R_2$. Now, since
    $R_1$ and $R_2$ are rings, we have that, since $x\in R_1$ and $y\in R_2$, $-x\in R_1$ and
    $-y\in R_2$. So, $(-x,-y)\in R_1\times R_2$. Hence
    
    $$(x,y)+(-x,-y)=(x+_1(-x),y+_2(-y))=(0_1,0_2)=(-x+_1x,-y+_2y)=(-x,-y)+(x,y)$$
    
    Therefore $R_1\times R_2$ is closed under additive inverses. Next, let
    $(a,b),(c,d)\in R_1\times R_2$. Thus,
    
    $$(a,b)+(c,d)=(a+_1c,b+_2d)=(c+_1a,d+_2b)=(c,d)+(a,b)$$
    
    by $(R_1,+_1)$ and $(R_2,+_2)$ being abelian. So, $(R_1\times R_2,+)$ is an abelian group. Now, let
    $(a,b),(c,d),(e,f)\in R_1\times R_2$. Then
    
    $$((a,b)\cdot(c,d))\cdot(e,f)=(a\cdot_1c,b\cdot_2d)\cdot(e,f)$$
    $$=((a\cdot_1c)\cdot_1e,(b\cdot_2d)\cdot_2f)=(a\cdot_1(c\cdot_1e),b\cdot_2(d\cdot_2f))$$
    $$=(a,b)\cdot(c\cdot_1e,d\cdot_2f)=(a,b)\cdot((c,d)\cdot(e,f))$$
    
    by associativity of multiplication on $R_1$ and $R_2$. Finally, let
    $(a,b),(c,d),(e,f)\in R_1\times R_2$. Therefore
    
    $$(a,b)\cdot((c,d)+(e,f))=(a,b)\cdot(c+_1e,d+_2f)=(a\cdot_1(c+_1e),b\cdot_2(d+_2f))$$
    $$=(a\cdot_1c+_1a\cdot_1e,b\cdot_2d+_2b\cdot_2f)$$
    
    and
    
    $$((c,d)+(e,f))\cdot(a,b)=(c+_1e,d+_2f)\cdot(a,b)=((c+_1e)\cdot_1a,(d+_2f)\cdot_2b)$$
    $$=(c\cdot_1a+_1e\cdot_1a,d\cdot_2b+_2f\cdot_2b)$$
    
    since $R_1$ and $R_2$ are rings. Thus $(a,b),(c,d),(e,f)\in R_1\times R_2$ is also a ring as
    desired.

\end{solution}