a. Apply the trapezoidal method to the equation $u'=\lambda u$ and show that

$$U^{n+1}=(\frac{1+z/2}{1-z/2})U^n$$

where $z=k\lambda$.\\

b. Let

$$R(z)=\frac{1+z/2}{1-z/2}$$

Show that $R(z)=e^z+\mathcal{O}(z^3)$ and conclude that the one-step error of the trapezoidal method
on this problem is $\mathcal{O}(k^3)$.\\

\begin{solution}\renewcommand{\qedsymbol}{}\ \\
    a. We have that the trapezoidal method is given by

    $$U^{n+1}=U^n+\frac{k}{2}(f(U^n)+f(U^{n=1}))$$

    Using $u'=\lambda u=f(u)$, we see that

    $$U^{n+1}=U^n+\frac{k}{2}(\lambda U^n+\lambda U^{n+1})$$
    $$=U^n+\frac{k\lambda}{2}U^n+\frac{k\lambda}{2}U^{n+1}$$
    $$U^n\frac{z}{2}U^n+\frac{z}{2}U^{n+1}$$

    Hence,

    $$U^{n+1}-\frac{z}{2}U^{n+1}=U^n+\frac{z}{2}U^n$$

    Therefore,

    $$(1-\frac{z}{2})U^{n+1}=(1+\frac{z}{2})U^n$$

    Thus,

    $$U^{n+1}=(\frac{1+z/2}{1-z/2})U^n$$

    as desired.\\

    b. Let $R(Z)$ be as given above. Note that the Taylor series expansion of $e^z$ about 0 is
    $e^z=1+z+\frac{z^2}{2}+\ldots$. Now, we are given the Neumann series
    $\frac{1}{1-z/2}=1+\frac{z}{2}+\frac{z^2}{4}+\frac{z^3}{8}+\ldots$. So,

    $$R(z)=(1+z/2)(\frac{1}{1-z/2})=(1+z/2)(1+\frac{z}{2}+\frac{z^2}{4}+\frac{z^3}{8}+\ldots)$$
    $$=1+\frac{z}{2}+\frac{z}{2}+\frac{z^2}{4}+\frac{z^2}{4}+\frac{z^3}{8}+\frac{z^3}{8}+\ldots$$

    $$=1+z+\frac{z^2}{2}+\mathcal{O}(z^3)=e^z+\mathcal{O}(z^3)$$

    Hence, we see that the one-step error of the trapezoidal method on this problem is
    $\mathcal{O}(k^3)$ as desired.

\end{solution}