Determine the characteristic polynomials $\rho(\zeta)$ and $\sigma(\zeta)$ for the following
linear multistep methods. Verify that (5.48) holds in each case.\\
a. The 3-step Adams-Bashforth method.\\
b. The 3-step Adams-Moulton method.\\
c. The 2-step Simpson's method of Example 5.16.\\

\begin{solution}\renewcommand{\qedsymbol}{}\ \\
    a. We have that the 3-step Adams-Bashforth method is given by

    $$U^{n+3}=U^{n+2}+\frac{h}{12}(5f(U^n)-16f(U^{n+1})+23f(U^{n+2}))$$

    Hence

    $$U^{n+3}-U^{n+2}=\frac{h}{12}(5f(U^n)-16f(U^{n+1})+23f(U^{n+2}))$$

    So, the characteristic polynomials are given by

    $$\rho(\zeta)=\zeta^3-\zeta^2$$
    $$\sigma(\zeta)=\frac{23}{12}\zeta^2-\frac43\zeta+\frac{5}{12}$$

    Now, we see that

    $$\sum_{j=0}^r\alpha_j=1+(-1)+0+0=0$$
    $$\sum_{j=0}^r\beta_j=\frac{23}{12}-\frac43+\frac{5}{12}=1=3(1)+2(-1)=\sum_{j=0}^rj\alpha_j$$

    Thus, condition (5.48) holds.\\

    b. We have that the 3-step Adams-Moulton method is given by

    $$U^{n+3}=U^{n+2}+\frac{h}{24}(f(U^n)-5f(U^{n+1})+19f(U^{n+2})+9f(U^{n+3}))$$

    Hence

    $$U^{n+3}-U^{n+2}=\frac{h}{24}(f(U^n)-5f(U^{n+1})+19f(U^{n+2})+9f(U^{n+3}))$$
    
    So, the characteristic polynomials are given by

    $$\rho(\zeta)=\zeta^3-\zeta^2$$
    $$\sigma(\zeta)=\frac38\zeta^3+\frac{19}{24}\zeta^2-\frac{5}{24}\zeta+\frac{1}{24}$$

    Now, we see that

    $$\sum_{j=0}^r\alpha_j=1+(-1)+0+0=0$$
    $$\sum_{j=0}^r\beta_j=\frac{3}{8}+\frac{19}{24}-\frac{5}{24}+\frac{1}{24}=1=3(1)+2(-1)=
    \sum_{j=0}^rj\alpha_j$$

    Thus, condition (5.48) holds.\\

    c. We have that the 2-step Simpson's method is given by

    $$U^{n+2}=U^{n}+\frac{2h}{6}(f(U^n)+4f(U^{n+1})+f(U^{n+2}))$$

    Hence

    $$U^{n+2}-U^{n}=\frac{2h}{6}(f(U^n)+4f(U^{n+1})+f(U^{n+2}))$$

    So, the characteristic polynomials are given by

    $$\rho(\zeta)=\zeta^2-1,\;\; \sigma(\zeta)=\frac13\zeta^2+\frac43\zeta+\frac13$$

    Now, we see that

    $$\sum_{j=0}^r\alpha_j=1+0-1=0$$
    $$\sum_{j=0}^r\beta_j=\frac{1}{3}+\frac43+\frac{1}{3}=2=2(1)+0(-1)=\sum_{j=0}^rj\alpha_j$$

    Thus, condition (5.48) holds.

\end{solution}