Let $(G,*)$ and $(H,\triangle)$ be groups and suppose that $f:G\rightarrow H$ is a homomorphism. Prove
that for any $g\in G$, $f(g^n)=(f(g))^n$ for all $n\in\mathbb{Z}^+$.\\\\

\begin{solution}\renewcommand{\qedsymbol}{}\ \\
    Let $G, H$, and $f$ be as given. Now, let $g\in G$ and $n\in\mathbb{Z}+$. Assume first that $n=1$.
    Then $f(g^1)=f(g)=(f(g))^1$. Now, let $n\geq1$ and assume that $f(g^n)=(f(g))^n$. Then,
    
    $$f(g^{n+1})=f(g^n*g)=f(g^n)\triangle f(g)=(f(g))^n\triangle (f(g))^1=(f(g))^{n+1}$$
    
    since $f$ is a homomorphism. Since $g\in G$ was arbitrary, we have that for all $n\in\mathbb{Z}^+$,
    $f(g^n)=(f(g))^n$ for any $g\in G$.

\end{solution}