a. Let $G$ be a group and $H$ a subgroup of $G$. Define the relation $R$ on $G$ by
$R=\{(x,y)\in G\times G:xy^{-1}\in H\}$. Prove R is symmetric.\\

b. Prove $R$ is transitive.\\

c. Prove that for any $g\in G$, we have $[g]=Hg$.\\

\begin{solution}\renewcommand{\qedsymbol}{}\ \\
    Let $G, H$, and $R$ be as given. Let $x,y\in G$ and $(x,y)\in R$. That means $xy^{-1}\in H$. Since
    $H$ is a subgroup of $G$, we have that $x,y^{-1}\in H$. Hence $x^{-1},y\in H$. Therefore
    $yx^{-1}\in H$ and thus we have that $(y,x)\in R$.\\

    Let $G, H$, and $R$ be as given. Let $x,y,z\in G$ and let $(x,y),(y,z)\in R$. So, $xy^{-1}\in H$ and
    $yz^{-1}\in H$. Since $H$ is closed under the operation by being a subgroup of $G$, we have that
    $xy^{-1}yz^{-1}=xez^{-1}=xz^{-1}\in H$ Thus, $(x,z)\in R$ and $R$ is transitive.\\

    Let $G, H$, and $R$ be as given and let $g\in G$. Let $x\in [g]$. Then $x\in G$ and $(g,x)\in R$.
    So, $gx^{-1}\in H$. So, $h=gx^{-1}$ for some $h\in H$. Hence $x^{-1}=g^{-1}h$ and therefore,
    $x=(g^{-1}h)^{-1}=h^{-1}g$. Since $H$ is a subgroup of $G$, $h^{-1}\in H$. Thus $x\in Hg$. Now, let
    $x\in Hg$. Then $x=hg$ for some $h\in H$, and so $xg^{-1}=h\in H$. So, $(x,g)\in R$, and since $R$
    is symmetric, we have that $(g,x)\in R$. Thus, $x\in [g]$. Hence $[g]=Hg$ as desired.

\end{solution}