Let $G$ be a group and let $a,b\in G$. Prove that the order of $a*b$ is the same as the order of
$b*a$.\\\\

\begin{solution}\renewcommand{\qedsymbol}{}\ \\
    Let $G$, $a$, and $b$ be as given above. This will be a proof by cases. Assume first that $a*b$ has
    order $n$ for some $n\in\mathbb{Z}^+$. We will show that $b*a$ also has order $n$. Well,
    $(a*b)^n=e$, so
    
    $$(a*b)\ldots(a*b)\smash{\llap{$\underbrace{\phantom{(a*b)\ldots(a*b)}}_{\text{$n$ times}}$}}$$
    $$=\smash[b]{a*\! \underbrace{(b*a)\cdots(b*a)\,}_\text{$n-1$ times}}*b=e$$
    
    Then,
    
    $$\smash[b]{\! \underbrace{(b*a)\cdots(b*a)\,}_\text{$n-1$ times}}=a^{-1}*b^{-1}$$
    
    Hence,
    
    $$\smash[b]{a*\! \underbrace{(b*a)\cdots(b*a)\,}_\text{$n-2$ times}}*b=a^{-1}*b^{-1}$$
    
    Continuing in the same pattern,we get $e=(a^{-1}*b^{-1})^n$, therefore, $e=((b*a)^{-1})^n$. So, now
    assume by way of contradiction that $(b*a)$ has order $m<n$. Then, $(b*a)^m=e$. So,
    $((b*a)^m)^{-1}=e^{-1}=e$. Hence $((b*a)^{-1})^m=(a^{-1}*b^{-1})^m=e$. By the same process as above,
    we get $(a*b)^m=e$ which contradicts the leastness of $n$. On the other hand assume that $a*b$ has
    infinite order. Suppose by way of contradiction that $b*a$ has finite order n. Then, $(b*a)^n=e$.
    Thus, $((b*a)^n)^{-1}=e^{-1}=e$. Hence, $((b*a)^{-1})^n=(a^{-1}*b^{-1})^n=e$. By the exact same
    process as above, we get $(a*b)^n=e$ which contradicts the order of $a*b$. Thus, we have $a*b$ and
    $b*a$ have the same order.

\end{solution}