Let $G$ be a group and let $g\in G$. Prove that the order of $g$ is the same as the order of
$g^{-1}$.\\\\

\begin{solution}\renewcommand{\qedsymbol}{}\ \\
    Let $G$, and $g$ be as given above. This will be a proof by cases. First assume that $g$ has finite
    order. That is, assume that $g$ has order $n$ for some $n\in\mathbb{Z}^+$. We will show that
    $g^{-1}$ has order $n$. Since $g^n=e$, we have that $(g^n)^{-1}=e^{-1}$. Hence,
    $(g^n)^{-1}=g^{-n}=(g^{-1})^n=e^{-1}=e$. Now, assume by way of contradiction that $g^{-1}$ has order
    $m<n$. So, $(g^{-1})^m=e$ and by exponent rules, we have $(g^m)^{-1}=e$. Therefore,
    $((g^m)^{-1})^{-1}=g^m=e^{-1}=e$ which contradicts the leastness of $n$. On the other hand, assume
    that $g$ has infinite order. Suppose by way of contradiction that $g^{-1}$ has finite order
    $n\in\mathbb{Z}^+$. Well, then $(g^{-1})^n=e$. Hence, $(g^n)^{-1}=e$, and so
    $((g^n)^{-1})^{-1}=g^n=e^{-1}=e$ which contradicts the order of $g$. Thus, $g$ and $g^{-1}$ have the
    same order.

\end{solution}