Let $R$ be a ring, $M$ a left $R$-module, and $\phi:M\rightarrow M$ an $R$-module homomorphism such that
$\phi\circ\phi=\phi$. Show that $M=\phi(M)+\ker(\phi)$ and $\phi(M)\cap\ker(\phi)=\{0\}$.

\begin{solution}\renewcommand{\qedsymbol}{}\ \\
    Let $R, M,$ and $\phi$ be as given. We will first show that $\phi(M)\cap\ker(\phi)=\{0\}$. Since we
    showed $\phi(0)=0$ for an arbitrary left $R$-module homomorphism, we clearly have that
    $\{0\}\subseteq\phi(M)\cap\ker(\phi)$. Now, let $m\in\phi(M)\cap\ker(\phi)$. Then $\phi(m)=0$ and
    $m\in M$ such that $m=\phi(n)$ for some $n\in M$. Since $\phi\circ\phi=\phi$, we have that
    $\phi(\phi(n))=\phi(m)=0$ and $\phi(\phi(n))=\phi(n)$. So, $\phi(n)=m=0$. Thus we have that
    $m\in\{0\}$. Therefore $\phi(M)\cap\ker(\phi)=\{0\}$. Now we will show that $M=\phi(M)+\ker(\phi)$.
    Clearly, since $\phi(M),\ker(\phi)\subseteq M$ and $M$ is closed under addition,
    $\phi(M)+\ker(\phi)\subseteq M$. So, let $x\in M$. Now,
    $\phi(M)+\ker(\phi)=\{m+n|m\in\phi(M),n\in\ker(\phi)\}$. We need to show that $x=\phi(m)+n$ for some
    $\phi(m)+n\in\phi(M)+ker(\phi)$. Take $\phi(x)=\phi(\phi(m)+n)$. Since $\phi$ is a homomorphism, we
    have that $\phi(x)=\phi(\phi(m))+\phi(n)$. By our assumption of $\phi$, $\phi(x)=\phi(m)+\phi(n)$
    and since $n\in\ker(\phi)$, $\phi(x)=\phi(m)$. Thus, we have that $x\in\phi(M)+ker(\phi)$. Therefore
    $M=\phi(M)+ker(\phi)$ as desired.

\end{solution}