7. Let $R$ be a ring, $M$ a left $R$-module, and $A\subseteq B$ $R$-submodules of $M$. Prove that
$(M/A)/(B/A)\cong(M/B)$.

\begin{solution}\renewcommand{\qedsymbol}{}\ \\
    Let $R, M, A$ and $B$ be as given above. By theorem 8, we have that $M/A$ is a left $R$-module.
    Similarly, we have that $M/B$ is a left $R$-module. Now consider $\phi:(M/A)\rightarrow(M/B)$
    defined by $\phi(m+A)=m+B$. Let $a\in R$ and $m+A,n+A\in M/A$. Then we have that
    $\phi((m+A)+(n+A))=\phi((m+n)+A)=(m+n)+B=(m+B)+(n+B)=\phi(m+A)+\phi(n+A)$ by the definition of
    $\phi$ and M/A, M/B as a left $R$-modules. Also, $a\phi(m+A)=a(m+B)=(am)+B=\phi((am)+A)$ by the
    definition of the action on quotient modules and $\phi$. So, we have that $\phi$ is an $R$-module
    homomorphism. Now,
    $\phi(M/A)=\{m+B\in M/B|\text{there exists} m+A\in M/A such that \phi(m+A)=m+B\}=\{m+B|m\in M\}$.
    So, $\phi(M/A)=M/B$ by our definition of $\phi$. Further,
    $\ker(\phi)=\{m+A\in M/A|\phi(m+A)=0\}=\{m+A\in M/A|m+B=0\}=\{m+A|m\in B\}$.
    That is $\ker(\phi)=M/B$. Thus, by the Fundamental Homomorphism Theorem, we have that
    $(M/A)/(B/A)\cong(M/B)$ as desired.

\end{solution}