9. Let $R$ be a ring, $M$ a left $R$-module, $N_1,\ldots, N_n$ submodules of $M$, and
$\pi:N_1\times\cdots\times N_n\rightarrow N_1+\cdots+N_n$ defined by
$\pi(m_1,\ldots,m_n)=m_1+\cdots+m_n$. Prove that the statement $\pi$ is an isomorphism is equivalent
to $N_i\cap(N_1+\cdots+N_{i-1}+N_{i+1}+\cdots+N_n)=\{0\}$ for all $i\in\{1,\ldots,n\}$.

\begin{solution}\renewcommand{\qedsymbol}{}\ \\
    Let $R, M, N_i$ for $1\leq i\leq n$, and $\pi$ be as given. Assume first that
    $N_i\cap(N_1+\cdots+N_{i-1}+N_{i+1}+\cdots+N_n)=\{0\}$ for all $i\in\{1,\ldots,n\}$.Now, let
    $a\in R$ and $(x_1,\ldots,x_n),(y_1,\ldots,y_n)\in\prod_{i=1}^nN_i$. Then,
    
    $$\pi((x_1,\ldots,x_n)+(y_1,\ldots,y_n))=\pi((x_1+y_1,\ldots,x_n+y_n))$$
    $$=x_1+y_1+\cdots+x_n+y_n=x_1+\cdots+x_n+y_1+\cdots+y_n=\pi((x_1\ldots,x_n))+\pi((y_1,\ldots,y_n))$$

    since $\sum_{i=1}^nN_i$ is an abelian group by definition of being an $R$-module. Also,

    $$a\pi((x_1,\ldots,x_n))=a((x_1+\cdots+x_n))=ax_1+\cdots+ax_n$$
    $$=\pi((ax_1,\ldots,ax_n))=\pi(a(x_1,\ldots,x_n))$$
    
    by the definition of the action on $\sum_{i=1}^nN_i$. So, we have that $\pi$ is an $R$-module
    homomorphism. Now, let $z\in\sum_{i=1}^nN_i$. Then $z=z_1+\cdots+z_n$ where $z_i\in N_i$ for
    $1\leq i\leq n$. Hence, we have that $\pi((z_1,\ldots,z_n))=z_1+\cdots+z_n$ and so $\pi$ is onto.
    Now, with $(x_1,\ldots,x_n),(y_1,\ldots,y_n)\in\prod_{i=1}^nN_i$, assume that
    $\pi((x_1,\ldots,x_n))=\pi((y_1,\ldots,y_n))$. So,

    $$\pi((x_1,\ldots,x_n))-\pi((y_1,\ldots,y_n))=\pi((x_1,\ldots,x_n)-(y_1,\ldots,y_n))$$
    $$=\pi((x_1-y_1,\ldots,x_n-y_n))=0$$

    since $\pi$ is a homomorphism. Therefore,
    $x_1-y_1+\cdots+x_n-y_n=0=\underbrace{0+\cdots+0}_{n\;\text{times}}$. Since
    $N_i\cap(N_1+\cdots+N_{i-1}+N_{i+1}+\cdots+N_n)=\{0\}$ for all $i\in\{1,\ldots,n\}$, we have that
    $x_i\neq y_j$ for all $i\neq j$. Thus, $x_1-y_1+\cdots+x_n-y_n=x_1+\cdots+x_n-y_1-\cdots-y_n$ and so
    $x_1+\cdots+x_n=y_1+\cdots+y_n$. Therefore, $(x_1,\ldots,x_n)=(y_1,\ldots,y_n)$. Thus, we have that
    $\pi$ is an isomorphism. Now, assume that $\pi$ is an $R$-module isomorphism. Take
    $(0,\ldots,0)\in\prod_{i=1}^nN_i$. Then,
    $\pi(0,\ldots,0)=\underbrace{0+\cdots+0}_{n\;\text{times}}$.
    Since $\pi$ is an isomorphism, then $\pi$ is $1-1$. Hence, $\ker(\pi)=\{(0,\ldots,0)\}$. That is,
    there exists no $(x_1,\ldots,x_n),(y_1,\ldots,y_n)\in\prod_{i=1}^nN_i$ such that if
    $\pi((x_1,\ldots,x_n)-(y_1,\ldots,y_n))=0$, then $x_i=y_j$ for all $i\neq j$ with $1\leq i,j\leq n$.
    Hence, we have that $N_i\cap(N_1+\cdots+N_{i-1}+N_{i+1}+\cdots+N_n)=\{0\}$ for all
    $i\in\{1,\ldots,n\}$. Thus, the two statements are equivalent as desired.

\end{solution}