\documentclass[12pt]{article}
\usepackage{amsmath}
\usepackage{amssymb}
\usepackage{amsthm}
\usepackage{accents}
\usepackage{graphicx}
\setlength{\oddsidemargin}{0in}
\setlength{\textwidth}{6.5in}
\setlength{\topmargin}{-.55in}
\setlength{\textheight}{9in}
\pagestyle{empty}
\renewcommand \d{\displaystyle}
\begin{document}
\noindent Dallas Klumpe

\noindent Math 5820

\noindent HW 17

11.2.20.a. Fit an exponential curve to the data.\\
Given the data and the sums, we have that $b=\frac{10(137.97415)-(35)(41.35720)}{10(169)-(35)^2}=-0.145722$ and $\ln a=\frac{41.35720-(-0.145722)(35)}{10}=104.1409$. So, we have the exponetial curve $y=104.1409e^{-0.1457x}$.\\
b. Estimate the half life of $^{195}$Au--aurothiomalate.\\
Well, the half life would be $50\%$. So, $50=104.1409e^{-0.1457x}$. Hence $x=\frac{\ln(\frac{50}{104.1409})}{-0.1457}=5.0358$. That is, the half life of the gold in a persons blood is about 5.04 days.\\[20pt]

11.3.6. Prove that $\sum_{i=1}^n(y_i-\hat{\beta}_0-\hat{\beta}_1x_i)^2=\sum_{i=1}^ny_i^2-\hat{\beta}_0\sum_{i=1}^ny_i-\hat{\beta}_1\sum_{i=1}^ny_ix_i$.\\
Well, $\sum_{i=1}^n(y_i-\hat{\beta}_0-\hat{\beta}_1x_i)^2=\sum_{i=1}^n(y_i-(\bar{y}-\hat{\beta}_1\bar{x})-\hat{\beta}_1x_i)^2=\sum_{i=1}^n((y_i-\bar{y})-\hat{\beta}_1(x_i-\bar{x}))^2=\sum_{i=1}^n(y_i-\bar{y})^2+\hat{\beta}_1^2\sum_{i=1}^n(x_i-\bar{x})^2-2\hat{\beta}_1\sum_{i=1}^n(x_i-\bar{x})(y_i-\bar{y})=$ $$\sum_{i=1}^n(y_i-\bar{y})^2+\hat{\beta}_1(\frac{\sum_{i=1}^n(x_i-\bar{x})(y_i-\bar{y})}{\sum_{i=1}^n(x_i-\bar{x})^2})\sum_{i=1}^n(x_i-\bar{x})^2-2\hat{\beta}_1\sum_{i=1}^n(x_i-\bar{x})(y_i-\bar{y})=$$ $$\sum_{i=1}^n(y_i-\bar{y})^2-\hat{\beta}_1\sum_{i=1}^n(x_i-\bar{x})(y_i-\bar{y})=$$ $$\sum_{i=1}^ny_i^2-n\bar{y}^2-\hat{\beta}_1(\sum_{i=1}^nx_iy_i-\frac1n(\sum_{i=1}^nx_i)(\sum_{i=1}^ny_i))=$$ $$\sum_{i=1}^ny_i^2-\hat{\beta}_1\sum_{i=1}^nx_iy_i-n\bar{y}^2+\hat{\beta}_1\frac1n(\sum_{i=1}^nx_i)(\sum_{i=1}^ny_i)=$$ $$\sum_{i=1}^ny_i^2-\hat{\beta}_1\sum_{i=1}^nx_iy_i-(\bar{y}+\hat{\beta}_1\bar{x})(\sum_{i=1}^ny_i)=$$ $$\sum_{i=1}^ny_i^2-\hat{\beta}_0\sum_{i=1}^ny_i-\hat{\beta}_1\sum_{i=1}^ny_ix_i$$




\end{document}