(\#3 in 2.2) Prove or disprove the following: For $B\subseteq Y$ and $f:X\to Y$,
$f^{-1}(Y\backslash B)=X\backslash f^{-1}(B)$.\\\\

\begin{solution}\renewcommand{\qedsymbol}{}\ \\
    Prove: Let $B, X,$ and $Y$ be sets, $B\subseteq Y$, and $f:X\rightarrow Y$ be a function. First
    assume that $B=\emptyset$. Then $Y\setminus B=Y$. So,
    $f^{-1}(Y\setminus B)=f^{-1}(Y)=X=X\setminus f^{-1}(B)$. So, assume that $B\neq\emptyset$ Let
    $x\in f^{-1}(Y\backslash B)$. Then, we have that $f(x)\in Y\setminus B$. So, by definition,
    $f(x)\in Y$ and $f(x)\notin B$. Again by definition, $x\in X$ but $x\notin f^{-1}(B)$. Therefore
    $x\in X\backslash f^{-1}(B)$ and $f^{-1}(Y\backslash B)\subseteq X\backslash f^{-1}(B)$. On the
    other hand, assume $x\in X\backslash f^{-1}(B)$. Well, we have then that $x\in X$ and
    $x\notin f^{-1}(B)$. So, by definition, $f(x)\in Y$, but also $f(x)\notin B$ Thus,
    $f(x)\in Y\setminus B$ and so $x\in f^{-1}(Y\backslash B)$. Therefore
    $f^{-1}(Y\backslash B)=X\backslash f^{-1}(B)$ as desired.

\end{solution}