Let $f: A \to B$ and $g: C \to D$ be continuous functions. Define a map
$f\times g: A\times C \to B\times D$ by the equation

$$(f\times g)(a,c) = (f(a), g(c)).$$

Show that $f\times g$ is continuous.\\\\

\begin{solution}\renewcommand{\qedsymbol}{}\ \\
    Let $f, g$, and $f\times g$ be as given above. Let $\tau_A, \tau_B, \tau_C$, and $\tau_D$ be
    topologies on $A, B, C$, and $D$ respectively. Let $U$ be open in $B$. Now,
    $(p_B\circ(f\times g))^{-1}(U)=(f\times g)^{-1}(p_B^{-1}(U))=
    \{(a,c)\in A\times C|(f\times g)((a,c))=(f(a),g(c))\in p_B^{-1}(U)\}$ where $p_B^{-1}(U)$ is open
    in $B\times D$ since $p_B$ is continuous. Well,
    $p_B^{-1}(U)=\{(b,d)\in B\times D|p_B((b,d))=b\in U\}=U\times D$. So, $f(a)\in U$ and $g(c)\in D$
    imples that $a\in f^{-1}(U)$ and $c\in g^{-1}(D)=C$. Therefore,
    $(p_B\circ(f\times g))^{-1}(U)=f^{-1}(U)\times C$ and since $f$ is continuous, $f^{-1}(U)$ and
    hence $f^{-1}(U)\times C$ is open. So, we see that $(p_B\circ(f\times g))^{-1}(U)$ is open in
    $A\times C$. Hence, $p_B\circ(f\times g)$ is continuous. Now let $U$ be open in $D$. So,
    $(p_D\circ(f\times g))^{-1}(U)=(f\times g)^{-1}(p_D^{-1}(U))=\{(a,c)\in A\times C|(f\times g)((a,c))
    =(f(a),g(c))\in p_D^{-1}(U)\}$ where $p_D^{-1}(U)=B\times U$ is open in $B\times D$ since $p_D$ is
    continuous. Now, $f(a)\in B$ and $g(c)\in U$ gives us $a\in f^{-1}(B)=A$ and $c\in g^{-1}(U)$. Since
    $g$ is continuous, $g^{-1}(U)$ is open. Thus, $(p_D\circ(f\times g))^{-1}(U)=A\times g^{-1}(U)$
    which is open in $A\times C$. Thus, $p_D\circ(f\times g)$ is continuous, and so $(f\times g)$
    is continuous by theorem 5.2.2. 

\end{solution}