Let $X$ and $Y$ be sets, and suppose that $f:X\rightarrow Y$ is a bijection.\\

i) For any $h\in S_X$, prove that $f\circ h\circ f^{-1}\in S_Y$.\\

ii) Now consider the map $\varphi:S_X\rightarrow S_Y$ defined by $\varphi(h)=f\circ h\circ f^{-1}$.
Prove that $\varphi$ is an isomorphism.\\\\

\begin{solution}\renewcommand{\qedsymbol}{}\ \\
    Let $X, Y$, and $f$ be as given. Let $h\in S_Y$. Now, let $y\in Y$. Then clearly
    $f(h(f^{-1}(y)))\in Y$. So we need only show that $f\circ h\circ f^{-1}$ is bijective. Then, let
    $x,y\in Y$ and assume $f(h(f^{-1}(x)))=f(h(f^{-1}(y)))$. Since $f$ is injective,
    $h(f^{-1}(x))=h(f^{-1}(y))$. Now, since $h$ is one-to-one, we have that $f^{-1}(x)=f^{-1}(y)$.
    Similarly, since $f$ is bijective, so to is $f^{-1}$, and so $f^{-1}$ is injective, thus $x=y$. So,
    $f\circ h\circ f^{-1}$ is one-to-one. Now, let $y\in Y$. Since $f$ is onto, there exists $x\in X$
    such that $f(x)=y$. SInce $h$ is also surjective, there exists $w\in X$ such that $h(w)=x$. Finally,
    since $f$ is bijective, $f^{-1}$ is also bijective, so $f^{-1}$ is onto. Therefore there exists
    $v\in Y$ such that $f^{-1}(v)=w$. Thus $f(h(f^{-1}(v)))=y$ and so $f\circ h\circ f^{-1}$ is onto.
    Since $h$ is arbitrary, we have that $f\circ h\circ f^{-1}\in S_Y$ for any $h\in S_X$.\\

    Let $X, Y, f$, and $\varphi$ be as given. Now, let $g,h\in S_X$ and assume that
    $\varphi(g)=\varphi(h)$. Then
    
    $$f\circ g\circ f^{-1}=f\circ h\circ f^{-1}$$
    
    So,
    
    $$f^{-1}\circ f\circ g\circ f^{-1}\circ f=f^{-1}\circ f\circ h\circ f^{-1}\circ f$$
    
    and therefore
    
    $$\epsilon\circ g\circ\epsilon=g=h=\epsilon\circ h\circ\epsilon$$
    
    Thus $\varphi$ is one-to-one. Now, let $f\circ h\circ f^{-1}\in S_Y$. Since $h\in S_X$, we have that
    $\varphi(h)=f\circ h\circ f^{-1}$ and so $\varphi$ is onto. Thus $\varphi$ is bijective. Now, let
    $g,h\in S_X$. Then,
    
    $$\varphi(g\circ h)=f\circ (g\circ h)\circ f^{-1}=f\circ g\circ h\circ f^{-1}$$
    $$=f\circ g\circ\epsilon\circ h\circ f^{-1}$$
    $$=f\circ g\circ f^{-1}\circ f\circ h\circ f^{-1}=\varphi(g)\circ\varphi(h)$$
    
    Thus $\varphi$ is an isomorphism.

\end{solution}