Prove that $\forall m\forall n$($m-n$ is odd) where $m$ is even and $n$ is odd.\\\\

\begin{solution}\renewcommand{\qedsymbol}{}\ \\
    Let $m$ be an even integer and $n$ an odd integer. Show that difference of an even integer and an
    odd integer is odd. Since $m$ is even, $m=2k$ for some $k\in \mathbb{Z}$ and since $n$ is odd,
    $n=2j+1$ for some $j\in \mathbb{Z}$. First take $n-m$. This gives us
    
    $$n-m=(2j+1)-2k=2(j-k)+1$$
    
    which is odd by assumption 2. Now take $m-n$. This yields
    
    $$m-n=2k-(2j+1)=2k-(2j+1+2-2)=2k-(2(j+1)-1)=2(k-(j+1))+1$$
    
    which is also odd by assumption. Thus, the difference of an even integer and an odd integer is odd.

\end{solution}