Let $G$ be a group and let $x,y\in G$. Prove that if $x*y=e$ then $y*x=e$.\\\\

\begin{solution}\renewcommand{\qedsymbol}{}\ \\
    Let $G, x,$ and $y$ be as given. Assume that $x*y=e$. Since $G$ is a group, there exists $x^{-1}$
    such that $x^{-1}*x=e$. So, we have that $x^{-1}*(x*y)=(x^{-1}*x)*y=e*y=y=x^{-1}*e=x^{-1}$. Hence
    $y=x^{-1}$. Similarlly, $y^{-1}$ exists such that $y*y^{-1}=e$. Therefore
    $(x*y)*y^{-1}=x*(y*y^{-1})=x*e=x=e*y^{-1}=y^{-1}$, and so, $x=y^{-1}$. So,
    $x^{-1}*(x*y)*y^{-1}=x^{-1}*e*y^{-1}$. Hence, $(x^-1*x)*(y*y^{-1})=x^{-1}*y^{-1}$. Thus,
    $e*e=e=y*x$ as desired.

\end{solution}