Consider the group $S_3$ and the elements $f$ and $g$ given by

$$f=\left(\begin{array}{ccc} 1 & 2 & 3\\ 3 & 2 & 1\end{array}\right)$$

and

$$g=\left(\begin{array}{ccc} 1 & 2 & 3\\ 2 & 3 & 1\end{array}\right)$$

Express $f\circ g$ and $f^{-1}$ using this notation.\\\\

\begin{solution}\renewcommand{\qedsymbol}{}\ \\
    Well,
    
    $$f\circ g=f(g(x))=\left(\begin{array}{ccc} 1 & 2 & 3\\ 2 & 1 & 3\end{array}\right)$$
    
    Now,
    
    $$f^{-1}(x)=\left(\begin{array}{ccc} 1 & 2 & 3\\ 3 & 2 & 1\end{array}\right)$$

\end{solution}